src/ext_traversal/rppo.v
@@ -1,0 +1,180 @@
+Require Import Setoid.
+From hahn Require Import Hahn.
+From imm Require Import AuxDef Events Execution Execution_eco
+     imm_common imm_s imm_s_hb CombRelations.
+Require Import AuxRel AuxRel2.
+
+Set Implicit Arguments.
+
+Section RPPO.
+Variable G : execution.
+Variable WF : Wf G.
+Variable COM : complete G.
+Variable sc : relation actid.
+Variable IMMCON : imm_consistent G sc.
+
+Notation "'acts'" := G.(acts).
+Notation "'sb'" := G.(sb).
+Notation "'rmw'" := G.(rmw).
+Notation "'data'" := G.(data).
+Notation "'addr'" := G.(addr).
+Notation "'ctrl'" := G.(ctrl).
+Notation "'rmw_dep'" := G.(rmw_dep).
+Notation "'rf'" := G.(rf).
+Notation "'co'" := G.(co).
+Notation "'coe'" := G.(coe).
+Notation "'fr'" := G.(fr).
+
+Notation "'eco'" := G.(eco).
+
+Notation "'bob'" := G.(bob).
+Notation "'fwbob'" := G.(fwbob).
+Notation "'ppo'" := G.(ppo).
+Notation "'fre'" := G.(fre).
+Notation "'rfi'" := G.(rfi).
+Notation "'rfe'" := G.(rfe).
+Notation "'deps'" := G.(deps).
+Notation "'detour'" := G.(detour).
+Notation "'release'" := G.(release).
+Notation "'sw'" := G.(sw).
+Notation "'hb'" := G.(hb).
+
+Notation "'urr'" := (urr G sc).
+Notation "'c_acq'" := (c_acq G sc).
+Notation "'c_cur'" := (c_cur G sc).
+Notation "'c_rel'" := (c_rel G sc).
+Notation "'t_acq'" := (t_acq G sc).
+Notation "'t_cur'" := (t_cur G sc).
+Notation "'t_rel'" := (t_rel G sc).
+Notation "'S_tm'" := G.(S_tm).
+Notation "'S_tmr'" := G.(S_tmr).
+Notation "'msg_rel'" := (msg_rel G sc).
+
+Notation "'lab'" := G.(lab).
+Notation "'loc'" := (loc lab).
+Notation "'val'" := (val lab).
+Notation "'mod'" := (Events.mod lab).
+Notation "'same_loc'" := (same_loc lab).
+
+Notation "'E'" := G.(acts_set).
+Notation "'R'" := (fun x => is_true (is_r lab x)).
+Notation "'W'" := (fun x => is_true (is_w lab x)).
+Notation "'F'" := (fun x => is_true (is_f lab x)).
+Notation "'RW'" := (R ∪₁ W).
+Notation "'FR'" := (F ∪₁ R).
+Notation "'FW'" := (F ∪₁ W).
+Notation "'R_ex'" := (fun a => is_true (R_ex lab a)).
+Notation "'W_ex'" := (W_ex G).
+Notation "'W_ex_acq'" := (W_ex ∩₁ (fun a => is_true (is_xacq lab a))).
+
+Notation "'Init'" := (fun a => is_true (is_init a)).
+Notation "'Loc_' l" := (fun x => loc x = Some l) (at level 1).
+Notation "'Tid_' t" := (fun x => tid x = t) (at level 1).
+Notation "'W_' l" := (W ∩₁ Loc_ l) (at level 1).
+
+Notation "'Pln'" := (fun x => is_true (is_only_pln lab x)).
+Notation "'Rlx'" := (fun x => is_true (is_rlx lab x)).
+Notation "'Rel'" := (fun x => is_true (is_rel lab x)).
+Notation "'Acq'" := (fun x => is_true (is_acq lab x)).
+Notation "'Acqrel'" := (fun x => is_true (is_acqrel lab x)).
+Notation "'Sc'" := (fun x => is_true (is_sc lab x)).
+Notation "'Acq/Rel'" := (fun a => is_true (is_ra lab a)).
+
+(******************************************************************************)
+(** **   *)
+(******************************************************************************)
+
+Definition rppo := (ctrl ∪ addr;;sb^? ∪ rmw_dep^? ;; <| R_ex |> ;; sb) ;; <| W |>.
+
+Lemma rppo_in_ppo : rppo ⊆ ppo.
+Proof.
+  unfold rppo, imm_common.ppo. hahn_frame.
+  rewrite WF.(wf_ctrlD) at 1.
+  rewrite (dom_l WF.(wf_addrD)) at 1.
+  arewrite (rmw_dep^? ⨾ ⦗R_ex⦘ ⊆ ⦗R⦘ ;; rmw_dep^? ⨾ ⦗R_ex⦘).
+  { rewrite (dom_l WF.(wf_rmw_depD)) at 1.
+    arewrite (⦗R_ex⦘ ⊆ ⦗R⦘ ;; ⦗R_ex⦘) at 1.
+    { type_solver. }
+    basic_solver. }
+  rewrite <- !seq_union_r.
+  hahn_frame.
+  unionL.
+  1,2: rewrite <- ct_step; eauto with hahn.
+  rewrite <- cr_ct, <- ct_step.
+  apply seq_mori; eauto with hahn.
+Qed.
+
+(* TODO: move to a more appropriate place. *)
+Lemma rmw_sb_cr_W_in_ppo : rmw ⨾ sb^? ⨾ ⦗W⦘ ⊆ ppo.
+Proof.
+  rewrite crE. rewrite seq_union_l, seq_union_r, seq_id_l.
+  rewrite WF.(rmw_sb_W_in_ppo).
+  rewrite WF.(rmw_in_ppo). eauto with hahn hahn_full.
+Qed.
+
+Lemma rppo_in_sb : rppo ⊆ sb.
+Proof. by rewrite rppo_in_ppo, ppo_in_sb. Qed.
+
+Lemma rppo_sb_in_rppo : rppo ;; sb ;; <|W|> ⊆ rppo.
+Proof.
+  unfold rppo.
+  hahn_frame. arewrite_id ⦗W⦘. rewrite seq_id_l.
+  rewrite !seq_union_l, !seqA.
+  rewrite WF.(ctrl_sb).
+  arewrite (sb^? ⨾ sb ⊆ sb^?).
+  { generalize (@sb_trans G). basic_solver. }
+  arewrite (sb ⨾ sb ⊆ sb).
+  2: done.
+  apply transitiveI. apply sb_trans.
+Qed.
+
+Lemma rppo_cr_sb_in_rppo : rppo ;; sb^? ;; <|W|> ⊆ rppo.
+Proof.
+  rewrite crE. rewrite seq_union_l, seq_union_r. rewrite rppo_sb_in_rppo.
+  basic_solver.
+Qed.
+
+Lemma data_rfi_rppo_in_ppo : ⦗R⦘ ⨾ (data ∪ rfi)＊ ⨾ rppo ⊆ ppo.
+Proof.
+  unfold rppo, imm_common.ppo.
+  hahn_frame.
+  rewrite <- rt_ct.
+  apply seq_mori.
+  { apply clos_refl_trans_mori; eauto 10 with hahn. }
+  unionL.
+  1,2: by rewrite <- ct_step; eauto 10 with hahn.
+  rewrite <- cr_ct, <- ct_step.
+  basic_solver 10.
+Qed.
+
+Lemma detour_rfe_data_rfi_rppo_in_detour_rfe_ppo :
+  (detour ∪ rfe) ⨾ (data ∪ rfi)＊ ⨾ rppo ⊆ (detour ∪ rfe) ⨾ ppo.
+Proof.
+  rewrite (dom_r WF.(wf_detourD)) at 1.
+  rewrite (dom_r WF.(wf_rfeD)) at 1.
+  rewrite <- seq_union_l, !seqA.
+    by rewrite data_rfi_rppo_in_ppo.
+Qed.
+
+Lemma rmw_in_rppo : rmw ⊆ rppo.
+Proof.
+  rewrite WF.(wf_rmwD), WF.(rmw_in_sb).
+  unfold rppo. basic_solver 10.
+Qed.
+
+Lemma rmw_sb_W_in_rppo : rmw ⨾ sb ⨾ ⦗W⦘ ⊆ rppo.
+Proof.
+  rewrite (dom_l WF.(wf_rmwD)), WF.(rmw_in_sb), !seqA.
+  arewrite (sb ⨾ sb ⊆ sb).
+  { apply transitiveI. apply sb_trans. }
+  unfold rppo. basic_solver 10.
+Qed.
+
+Lemma rmw_sb_cr_W_in_rppo : rmw ⨾ sb^? ⨾ ⦗W⦘ ⊆ rppo.
+Proof.
+  rewrite crE. rewrite seq_union_l, seq_union_r, seq_id_l.
+  rewrite rmw_sb_W_in_rppo.
+  rewrite rmw_in_rppo. eauto with hahn hahn_full.
+Qed.
+
+End RPPO.
